Refinement cleanup

Refinement.thy
@@ -2,6 +2,78 @@ theory Refinement
   imports "Collections.Refine_Dflt_Only_ICF" LayerMaintenance
 begin
 
+subsection \<open>PathFinding\<close>
+
+context Graph
+begin
+definition pathFindingRefine :: "node \<Rightarrow> path nres" where
+  "pathFindingRefine s \<equiv> do {
+    (p, _) \<leftarrow> WHILE (\<lambda>(p, u). outgoing u \<noteq> {}) (\<lambda>(p, u). do {
+      e \<leftarrow> SPEC (\<lambda>e. e \<in> outgoing u);
+      let p = p @ [e];
+      let u = snd e;
+      RETURN (p, u)
+    }) ([], s);
+    RETURN p
+  }"
+
+definition pathFinding_invar :: "node \<Rightarrow> (path \<times> node) \<Rightarrow> bool" where
+  "pathFinding_invar s \<equiv> \<lambda>(p, u). isPath s p u"
+
+lemma pathFinding_invar_step:
+  "\<lbrakk>e \<in> outgoing u; pathFinding_invar s (p, u)\<rbrakk> \<Longrightarrow> pathFinding_invar s (p @ [e], snd e)"
+  unfolding pathFinding_invar_def by (auto simp: isPath_tail outgoing_def)
+
+lemma pathFinding_finds_maximal_path: "pathFindingRefine s \<le> SPEC (\<lambda>p. \<exists>u. outgoing u = {} \<and> isPath s p u)"
+  unfolding pathFindingRefine_def
+  apply (intro WHILE_rule[where I="pathFinding_invar s"] refine_vcg)
+    apply (auto intro: pathFinding_invar_step)
+  unfolding pathFinding_invar_def by auto
+end \<comment> \<open>Graph\<close>
+
+context ST_Graph
+begin
+(* TODO useful? then move *)
+lemma stl_no_outD: "stl.outgoing u = {} \<Longrightarrow> u = t \<or> u \<notin> stl.V"
+  using only_t_without_stl_outgoing by blast
+
+
+find_theorems "(?A :: _ nres) \<le> ?B \<Longrightarrow> ?B \<le> ?C \<Longrightarrow> ?A \<le> ?C"
+thm SPEC_trans
+thm nrec.leq_trans
+
+
+find_theorems "SPEC ?A \<le> SPEC ?B"
+thm SPEC_rule
+thm iSPEC_rule
+(* TODO why are there two? *)
+
+lemma pathFinding_finds_st_path:
+  assumes "connected s t"
+  shows "stl.pathFindingRefine s \<le> SPEC (\<lambda>p. isPath s p t)"
+proof (rule nrec.leq_trans[OF stl.pathFinding_finds_maximal_path], rule SPEC_rule)
+  fix p
+  assume "\<exists>u. stl.outgoing u = {} \<and> stl.isPath s p u"
+  then obtain u where NO_OUT: "stl.outgoing u = {}" and PATH: "stl.isPath s p u" by blast
+  then have "u = t \<or> u \<notin> stl.V" using stl_no_outD by simp
+  with PATH show "isPath s p t"
+  proof (elim disjE)
+    assume "u \<notin> stl.V"
+    with PATH have "u = s" "p = []"
+      using stl.acyclic stl.isCycle_def
+      by (metis stl.connected_def stl.distinct_nodes_in_V_if_connected(2))+
+    with NO_OUT have "s = t \<or> s \<notin> stl.V" using stl_no_outD by blast
+    with assms have "s = t"
+      using stl.distinct_nodes_in_V_if_connected stl_maintains_st_connected by blast
+    with \<open>p = []\<close> show ?thesis by simp
+  qed (auto intro: stl_sub_c.sg_paths_are_base_paths)
+qed (* TODO prettify *)
+end \<comment> \<open>ST_Graph\<close>
+
+\<comment> \<open>PathFinding\<close>
+
+subsection \<open>RightPass\<close>
+
 definition removeEdge :: "_ graph \<Rightarrow> edge \<Rightarrow> _ graph" where
   "removeEdge c e \<equiv> c(e := 0)"
 
@@ -21,134 +93,6 @@ definition rightPassRefine :: "_ graph \<Rightarrow> edge set \<Rightarrow> (_ g
     RETURN c
   }"
 
-(*
-definition pathFindingRefine :: "_ graph  \<Rightarrow> node \<Rightarrow> path nres" where
-  "pathFindingRefine c s \<equiv> do {
-    (p, _) \<leftarrow> WHILE (\<lambda>(p, u). Graph.outgoing c u \<noteq> {}) (\<lambda>(p, u). do {
-      e \<leftarrow> SPEC (\<lambda>e. e \<in> Graph.outgoing c u);
-      let p = p @ [e];
-      let u = snd e;
-      RETURN (p, u)
-    }) ([], s);
-    RETURN p
-  }"
-
-definition pathFinding_invar :: "_ graph \<Rightarrow> node \<Rightarrow> (path \<times> node) \<Rightarrow> bool" where
-  "pathFinding_invar c s \<equiv> \<lambda>(p, u). Graph.isPath c s p u"
-
-lemma pathFinding_invar_step:
-  "\<lbrakk>e \<in> Graph.outgoing c u; pathFinding_invar c s (p, u)\<rbrakk> \<Longrightarrow> pathFinding_invar c s (p @ [e], snd e)"
-  unfolding pathFinding_invar_def using Graph.isPath_tail Graph.outgoing_def
-  by (smt (verit, best) case_prod_conv fst_conv mem_Collect_eq)
-
-lemma pathFinding_finds_path: "pathFindingRefine c s \<le> SPEC (\<lambda>p. \<exists>u. Graph.isPath c s p u)"
-  unfolding pathFindingRefine_def
-  apply (intro WHILE_rule[where I="pathFinding_invar c s"] refine_vcg)
-    apply (auto intro: pathFinding_invar_step)
-  unfolding pathFinding_invar_def
-   apply (auto simp: Graph.isPath.simps)
-  done
-*)
-
-thm it_step_insert_iff
-
-
-context Graph
-begin
-definition pathFindingRefine :: "node \<Rightarrow> path nres" where
-  "pathFindingRefine s \<equiv> do {
-    (p, _) \<leftarrow> WHILE (\<lambda>(p, u). outgoing u \<noteq> {}) (\<lambda>(p, u). do {
-      e \<leftarrow> SPEC (\<lambda>e. e \<in> outgoing u);
-      let p = p @ [e];
-      let u = snd e;
-      RETURN (p, u)
-    }) ([], s);
-    RETURN p
-  }"
-
-definition pathFinding_invar :: "node \<Rightarrow> (path \<times> node) \<Rightarrow> bool" where
-  "pathFinding_invar s \<equiv> \<lambda>(p, u). isPath s p u"
-
-(*
-lemma pathFinding_invar_step:
-  "\<lbrakk>e \<in> outgoing u; pathFinding_invar s (p, u)\<rbrakk> \<Longrightarrow> pathFinding_invar s (p @ [e], snd e) \<and> snd e \<in> V"
-  unfolding pathFinding_invar_def V_def using isPath_tail outgoing_def by fastforce
-*)
-
-lemma pathFinding_invar_step:
-  "\<lbrakk>e \<in> outgoing u; pathFinding_invar s (p, u)\<rbrakk> \<Longrightarrow> pathFinding_invar s (p @ [e], snd e)"
-  unfolding pathFinding_invar_def by (auto simp: isPath_tail outgoing_def)
-
-lemma tmp: 
-  "\<lbrakk>e \<in> outgoing u; pathFinding_invar s (p, u)\<rbrakk> \<Longrightarrow> snd e \<in> V"
-  unfolding pathFinding_invar_def V_def using outgoing_def by fastforce
-
-lemma pathFinding_finds_path: "pathFindingRefine s \<le> SPEC (\<lambda>p. \<exists>u. isPath s p u)"
-  unfolding pathFindingRefine_def
-  apply (intro WHILE_rule[where I="pathFinding_invar s"] refine_vcg)
-    apply (auto intro: pathFinding_invar_step)
-  unfolding pathFinding_invar_def by auto
-end
-
-thm if_split
-thm case_split
-
-(*
-lemma (in Graph) tmp':
-  assumes "isPath u p v" "v \<notin> V"
-  obtains "u \<notin> V" "p = []"
-  using assms sledgehammer
-*)
-
-context ST_Graph
-begin
-(* TODO useful? then move *)
-lemma stl_no_outD: "stl.outgoing u = {} \<Longrightarrow> u = t \<or> u \<notin> stl.V"
-  using only_t_without_stl_outgoing by blast
-
-
-lemma pathFinding_finds_st_path:
-  assumes "connected s t"
-  shows "stl.pathFindingRefine s \<le> SPEC (\<lambda>p. isPath s p t)"
-  unfolding stl.pathFindingRefine_def
-proof (intro WHILE_rule[where I="stl.pathFinding_invar s"] refine_vcg, simp_all)
-  show "stl.pathFinding_invar s ([], s)" unfolding stl.pathFinding_invar_def by simp
-next
-  fix p u e
-  assume "e \<in> stl.outgoing u" "stl.pathFinding_invar s (p, u)"
-  then show "stl.pathFinding_invar s (p @ [e], snd e)" by (rule stl.pathFinding_invar_step)
-next
-  fix p u
-  assume "stl.outgoing u = {}" "stl.pathFinding_invar s (p, u)"
-  then have "u = t \<or> u \<notin> stl.V" "stl.isPath s p u" unfolding stl.pathFinding_invar_def
-    using stl_no_outD by auto
-  then show "isPath s p t"
-  proof (elim disjE)
-    assume "u = t"
-    with \<open>stl.isPath s p u\<close> show "isPath s p t" using stl_sub_c.sg_paths_are_base_paths by blast
-  next
-    assume "u \<notin> stl.V"
-    with \<open>stl.isPath s p u\<close> have "u = s" "p = []"
-      using stl.acyclic stl.isCycle_def
-      by (metis stl.connected_def stl.distinct_nodes_in_V_if_connected(2))+
-    with \<open>stl.outgoing u = {}\<close> have "s = t \<or> s \<notin> stl.V" using stl_no_outD by blast
-    with assms have "s = t"
-      using stl.distinct_nodes_in_V_if_connected stl_maintains_st_connected by blast
-    with \<open>p = []\<close> show ?thesis by simp
-  qed
-qed (* TODO prettify *)
-end
-
-
-
-
-
-(* v \<leftarrow> SPEC (\<lambda>v. v \<in> snd ` Q); *)
-
-
-find_consts "'a set \<Rightarrow> 'a \<Rightarrow> bool"
-thm contains_def
-thm if_split
-thm prod.splits
+\<comment> \<open>RightPass\<close>
 
 end
